refine: add IRQReserved to state relation
Previously, irq_state_relation did not admit reserved IRQs. This was
addressed in arm-hyp but not standardised across other architectures,
and subsequently overwritten during arch-split efforts.

Signed-off-by: Ryan Barry <ryan.barry@proofcraft.systems>

proof/refine/StateRelation.thy
@@ -263,6 +263,7 @@ definition irq_state_relation :: "irq_state \<Rightarrow> irqstate \<Rightarrow>
      (irq_state.IRQInactive, irqstate.IRQInactive) \<Rightarrow> True
    | (irq_state.IRQSignal, irqstate.IRQSignal) \<Rightarrow> True
    | (irq_state.IRQTimer, irqstate.IRQTimer) \<Rightarrow> True
+   | (irq_state.IRQReserved, irqstate.IRQReserved) \<Rightarrow> True
    | _ \<Rightarrow> False"
 
 definition interrupt_state_relation ::
