proof/refine/ARM_HYP/ArchMachine_R.thy
@@ -69,5 +69,14 @@ lemma getActiveIRQ_le_maxIRQ:
   apply (simp add: irqs_masked'_def valid_irq_states'_def)
   done
 
+lemma doMachineOp_getActiveIRQ_non_kernel[wp]:
+  "\<lbrace>\<top>\<rbrace> doMachineOp (getActiveIRQ True)
+   \<lbrace>\<lambda>rv s. \<forall>irq. rv = Some irq \<longrightarrow> irq \<in> non_kernel_IRQs \<longrightarrow> P irq s\<rbrace>"
+  unfolding doMachineOp_def
+  apply wpsimp
+  apply (drule use_valid, rule getActiveIRQ_neq_non_kernel, rule TrueI)
+  apply clarsimp
+  done
+
 end
 end
